atomics/general_atomics.v
@@ -1,7 +1,7 @@
- From VST.veric Require Import rmaps compcert_rmaps.
+From VST.veric Require Import rmaps compcert_rmaps.
 Require Export iris.bi.lib.atomic.
 Require Export VST.veric.bi.
-From VST.concurrency Require Import ghosts conclib invariants fupd.
+From VST.concurrency Require Export ghosts conclib invariants fupd.
 Require Import VST.floyd.library.
 Require Export VST.zlist.sublist.
 Require Import Program.Equality.
