progs64/verif_incr.v
@@ -98,11 +98,11 @@ Proof.
   destruct left.
   - rewrite sepcon_assoc, (sepcon_comm _ (ghost_var _ _ _)), <- sepcon_assoc.
     erewrite ghost_var_share_join' by eauto with share.
-    Intros; rewrite prop_true_andp by auto; eapply derives_trans, fupd_frame_r; cancel.
-    eapply derives_trans, bupd_fupd; apply ghost_var_update.
+    Intros; rewrite prop_true_andp by auto; eapply derives_trans, bupd_frame_r; cancel.
+    apply ghost_var_update.
   - erewrite sepcon_assoc, ghost_var_share_join' by eauto with share.
-    Intros; rewrite prop_true_andp by auto; eapply derives_trans, fupd_frame_r; cancel.
-    eapply derives_trans, bupd_fupd; apply ghost_var_update.
+    Intros; rewrite prop_true_andp by auto; eapply derives_trans, bupd_frame_r; cancel.
+    apply ghost_var_update.
 Qed.
 #[export] Hint Resolve thread_inv_exclusive : core.
 
@@ -121,14 +121,8 @@ Proof.
   viewshift_SEP 0 (!!((if left then x else y) = n) && ghost_var Tsh (n+1) (if left then g1 else g2) *
     ghost_var gsh1 (if left then y else x) (if left then g2 else g1)).
   { go_lower.
-    destruct left.
-    - rewrite (sepcon_comm _ (ghost_var _ _ _)), <- sepcon_assoc.
-      erewrite ghost_var_share_join' by eauto with share.
-      Intros; rewrite prop_true_andp by auto; eapply derives_trans, bupd_frame_r; cancel.
-      apply ghost_var_update.
-    - erewrite ghost_var_share_join' by eauto with share.
-      Intros; rewrite prop_true_andp by auto; eapply derives_trans, bupd_frame_r; cancel.
-      apply ghost_var_update. }
+    eapply derives_trans, bupd_fupd.
+    rewrite <- sepcon_assoc; apply ghost_var_incr. }
   Intros; forward_call (gv _ctr_lock, sh, cptr_lock_inv g1 g2 (gv _ctr)).
   { lock_props.
     unfold cptr_lock_inv; Exists (z + 1).
